WiP: made LiveModel an instance of FairModel with tids as roles

fairness/examples/spinlock/spinlock_sc_comp_model.v
@@ -1,4 +1,5 @@
 From trillium.fairness.examples.spinlock Require Import spinlock_sc.
+From trillium.fairness Require Import fairness. 
 
 
 Close Scope Z_scope.
@@ -9,6 +10,62 @@ Opaque program.
 Opaque program_init_fuels.
 Opaque spinlock_model_impl. 
 Opaque sm_fuel. 
+
+Section LMFair.
+  Context `{LM: LiveModel Λ M}.
+  Context `{Countable (locale Λ), Inhabited (locale Λ)}.
+  Context `{Inhabited (fmstate M)}.
+
+  Definition locale_trans (st1: lm_ls LM) (τ: locale Λ) st2 :=
+    ls_trans (lm_fl LM) st1 (Silent_step τ) st2 \/
+    exists ρ, ls_trans (lm_fl LM) st1 (Take_step ρ τ) st2. 
+
+  Instance locale_trans_ex_dec τ st1:
+    Decision (exists st2, locale_trans st1 τ st2).
+  Proof.
+    (* intros.  *)
+  Admitted.
+
+  Lemma lm_ls_eqdec: EqDecision (lm_ls LM).
+  Proof. Admitted. 
+
+  Definition LM_Fair: FairModel.
+    refine {|
+        fmstate := lm_ls LM;
+        fmrole := locale Λ;
+        fmtrans :=
+          fun st1 oρ st2 => 
+            match oρ with
+            | Some τ => locale_trans st1 τ st2
+            | _ => False
+            end;
+        live_roles δ := filter (fun τ => exists δ', locale_trans δ τ δ') (map_img (ls_mapping δ));
+      |}.
+    - apply lm_ls_eqdec. 
+    - apply @inhabitant in H0 as l. apply @inhabitant in H1 as st.  
+      eapply populate. refine 
+        {| ls_under := st; 
+           ls_fuel := gset_to_gmap 0 (live_roles _ st);
+           ls_mapping := gset_to_gmap l (live_roles _ st); |}.
+      + by rewrite dom_gset_to_gmap.
+      + set_solver.
+    - intros ??? STEP.
+      apply elem_of_filter. split; eauto. 
+      inversion STEP as [[STEP']|[? STEP']]. 
+      + inversion STEP'. eapply elem_of_map_img; eauto.
+      + inversion STEP'. eapply elem_of_map_img; eauto.
+        destruct H3. eauto.
+  Defined. 
+
+  Lemma LM_live_roles_strong δ τ:
+    τ ∈ live_roles LM_Fair δ <-> (exists δ', locale_trans δ τ δ').
+  Proof. 
+    split.
+    2: { intros [??]. eapply LM_Fair. simpl. eauto. }
+    simpl. intros [??]%elem_of_filter. eauto.
+  Qed. 
+
+End LMFair.
 
 Section LocksCompositionModel.
 
